Move Bookstore.experimental.v to Bookstore.v.

examples/Bookstore.v
@@ -1,291 +1,126 @@
-Section BookStoreExamples.
-  Require Import QueryStructureNotations.
-  Require Import ListImplementation.
+Require Import AutoDB.
 
-  (* Our bookstore has two relations (tables):
-     - The [Books] relation contains the books in the
-       inventory, represented as a tuple with
-       [Author], [Title], and [ISBN] attributes.
-       The [ISBN] attribute is a key for the relation,
-       specified by the [where attributes .. depend on ..]
-       constraint.
-     - The [Orders] relation contains the orders that
-       have been placed, represented as a tuple with the
-       [ISBN] and [Date] attributes.
-
-     The schema for the entire query structure specifies that
-     the [ISBN] attribute of [Orders] is a foreign key into
-     [Books], specified by the [attribute .. of .. references ..]
+(* Our bookstore has two relations (tables):
+   - The [Books] relation contains the books in the
+     inventory, represented as a tuple with
+     [Author], [Title], and [ISBN] attributes.
+     The [ISBN] attribute is a key for the relation,
+     specified by the [where attributes .. depend on ..]
      constraint.
-   *)
+   - The [Orders] relation contains the orders that
+     have been placed, represented as a tuple with the
+     [ISBN] and [Date] attributes.
 
-  Definition BookStoreSchema :=
-    Query Structure Schema
-      [ relation "Books" has
-                schema <"Author" :: string,
-                        "Title" :: string,
-                        "ISBN" :: nat>
-                        where attributes ["Title"; "Author"] depend on ["ISBN"];
-        relation "Orders" has
-                schema <"ISBN" :: nat,
-                        "Date" :: nat> ]
-      enforcing [attribute "ISBN" for "Orders" references "Books"].
+   The schema for the entire query structure specifies that
+   the [ISBN] attribute of [Orders] is a foreign key into
+   [Books], specified by the [attribute .. of .. references ..]
+   constraint.
+ *)
 
-  (* Aliases for the tuples contained in Books and Orders, respectively. *)
-  Definition Book := TupleDef BookStoreSchema "Books".
-  Definition Order := TupleDef BookStoreSchema "Orders".
+(* Let's define some synonyms for strings we'll need,
+ * to save on type-checking time.
+ * (Thanks for being weird, Coq!) *)
+Definition sBOOKS := "Books".
+Definition sAUTHOR := "Authors".
+Definition sTITLE := "Title".
+Definition sISBN := "ISBN".
+Definition sORDERS := "Orders".
+Definition sDATE := "Date".
 
-  (* Our bookstore has two mutators:
-     - [PlaceOrder] : Place an order into the 'Orders' table
-     - [AddBook] : Add a book to the inventory
+(* Now here's the actual schema, in the usual sense. *)
+Definition BookStoreSchema :=
+  Query Structure Schema
+    [ relation sBOOKS has
+              schema <sAUTHOR :: string,
+                      sTITLE :: string,
+                      sISBN :: nat>
+              where attributes [sTITLE; sAUTHOR] depend on [sISBN];
+      relation sORDERS has
+              schema <sISBN :: nat,
+                      sDATE :: nat> ]
+    enforcing [attribute sISBN for sORDERS references sBOOKS].
 
-     Our bookstore has two observers:
-     - [GetTitles] : The titles of books written by a given author
-     - [NumOrders] : The number of orders for a given author
-   *)
+(* Aliases for the tuples contained in Books and Orders, respectively. *)
+Definition Book := TupleDef BookStoreSchema sBOOKS.
+Definition Order := TupleDef BookStoreSchema sORDERS.
 
-  Definition BookStoreSig : ADTSig :=
-    ADTsignature {
-        "InitBookstore" : unit → rep,
-        "PlaceOrder" : rep × Order → rep × bool,
-        "AddBook" : rep × Book → rep × bool,
-        "GetTitles" : rep × string → rep × list string,
-        "NumOrders" : rep × string → rep × nat
-      }.
+(* Our bookstore has two mutators:
+   - [PlaceOrder] : Place an order into the 'Orders' table
+   - [AddBook] : Add a book to the inventory
 
-  Definition BookStoreSpec : ADT BookStoreSig :=
-    QueryADTRep BookStoreSchema {
-      const "InitBookstore" (_ : unit) : rep := empty,
+   Our bookstore has two observers:
+   - [GetTitles] : The titles of books written by a given author
+   - [NumOrders] : The number of orders for a given author
+ *)
 
-      update "PlaceOrder" ( o : Order ) : bool :=
-          Insert o into "Orders",
+(* So, first let's give the type signatures of the methods. *)
+Definition BookStoreSig : ADTSig :=
+  ADTsignature {
+      "Init" : unit → rep,
+      "PlaceOrder" : rep × Order → rep × bool,
+      "AddBook" : rep × Book → rep × bool,
+      "GetTitles" : rep × string → rep × list string,
+      "NumOrders" : rep × string → rep × nat
+    }.
 
-      update "AddBook" ( b : Book ) : bool :=
-          Insert b into "Books" ,
+(* Now we write what the methods should actually do. *)
+Definition BookStoreSpec : ADT BookStoreSig :=
+  QueryADTRep BookStoreSchema {
+    const "Init" (_ : unit) : rep := empty,
 
-      query "GetTitles" ( author : string ) : list string :=
-        For (b in "Books")
-        Where (author = b!"Author")
-        Return (b!"Title"),
+    update "PlaceOrder" ( o : Order ) : bool :=
+        Insert o into sORDERS,
 
-       query "NumOrders" ( author : string ) : nat :=
-          Count (For (o in "Orders") (b in "Books")
-                 Where (author = b!"Author")
-                 Where (b!"ISBN" = o!"ISBN")
-                 Return o!"ISBN")
-  }.
+    update "AddBook" ( b : Book ) : bool :=
+        Insert b into sBOOKS ,
 
-  Require Import BagsOfTuples.
+    query "GetTitles" ( author : string ) : list string :=
+      For (b in sBOOKS)
+      Where (author = b!sAUTHOR)
+      Return (b!sTITLE),
 
-  Definition BookStoreListImpl_AbsR
-             (or : UnConstrQueryStructure BookStoreSchema)
-             (nr : list Book * list Order) : Prop :=
-    or ! "Books" ≃ benumerate (fst nr) /\ or ! "Orders" ≃ benumerate (snd nr).
+     query "NumOrders" ( author : string ) : nat :=
+        Count (For (o in sORDERS) (b in sBOOKS)
+               Where (author = b!sAUTHOR)
+               Where (b!sISBN = o!sISBN)
+               Return o!sISBN)
+}.
 
-  Opaque Query_For.
+(* Aliases for internal names of the two tables *)
+Definition Books := BookStoreSchema/sBOOKS. 
+Definition Orders := BookStoreSchema/sORDERS.
 
-  Definition BookStore :
-    Sharpened BookStoreSpec.
-  Proof.
-    unfold BookStoreSpec.
+(* Aliases for internal notions of schemas for the two tables *)
+Definition BookSchema := QSGetNRelSchemaHeading BookStoreSchema Books.
+Definition OrderSchema := QSGetNRelSchemaHeading BookStoreSchema Orders.
 
-    (* Step 1: Drop the constraints on the tables. From the perspective
-      of a client of a sharpened ADT the invariants will still hold,
-      since ADT refinement preserves the simulation relation. *)
+(* Now we define an index structure for each table. *)
 
-    start honing QueryStructure.
+Definition BookStorage : @BagPlusBagProof Book.
+  mkIndex BookSchema [ Books//sAUTHOR; Books//sISBN ].
+Defined.
+(* In other words, index first on the author field, then the ISBN field.
+ * Works especially efficiently for accesses keyed on author. *)
 
-    hone representation using BookStoreListImpl_AbsR.
+Definition OrderStorage : @BagPlusBagProof Order.
+  mkIndex OrderSchema [ Orders//sISBN ].
+Defined.
 
-    hone method "PlaceOrder".
-    {
-      rewrite refine_pick_val with (A := nat) (a := length (snd r_n)).
-      simplify with monad laws.
-      (* TODO: remove this etransitivity, apply step. *)
-      etransitivity.
-      apply refine_bind.
-      eapply (@refine_foreign_key_check
-                 _
-                 _ (fst r_n)
-      (fun tup2 : Tuple => n ``("ISBN") = tup2 ``("ISBN"))).
-      destruct H0; eauto.
-      unfold pointwise_relation; intros.
-      higher_order_1_reflexivity.
-      (* END TODO*)
-      pose_string_ids.
-      simplify with monad laws.
-      unfold If_Then_Else; rewrite refine_if_bool_eta.
-      simplify with monad laws.
-      unfold BookStoreListImpl_AbsR in *; split_and; simpl in *.
-      pose_string_ids.
-      rewrite refineEquiv_pick_pair.
-      simplify with monad laws; simpl.
-      Split Constraint Checks.
-      (* TODO move this back to a tactic *)
-      etransitivity.
-      subst_strings.
-      match goal with
-          |- context
-               [{a | EnsembleIndexedListEquivalence
-                       ((@UpdateUnConstrRelation ?QSSchema ?c ?Ridx
-                                                (EnsembleInsert ?n (?c!?R)))!?R')%QueryImpl a}%comp] =>
-          let H := fresh in
-          generalize ((@ImplementListInsert_neq QSSchema
-                                                {| bindex := R' |}
-                                                {| bindex := R |} n c)) as H; intros; setoid_rewrite H
-      end; try reflexivity; try eassumption.
-      congruence.
-      simplify with monad laws.
-      match goal with
-          |- context
-               [{a | EnsembleIndexedListEquivalence
-                       ((@UpdateUnConstrRelation ?QSSchema ?c ?Ridx
-                                                (EnsembleInsert ?n (?c!?R)))!?R)%QueryImpl a}%comp] =>
-          let H := fresh in
-          generalize ((@ImplementListInsert_eq QSSchema
-                                                {| bindex := R |}
-                                                n c)) as H; intros; setoid_rewrite H
-      end; try reflexivity; try eassumption.
-      rewrite refine_pick_val; eauto.
-      simplify with monad laws.
-      rewrite refine_pick_val; eauto.
-      simplify with monad laws.
-      reflexivity.
-      intros.
-      destruct H0 as [_ [l l']].
-      generalize (l _ H1).
-      unfold not; intros.
-      eapply lt_irrefl.
-      destruct tup; simpl in *; subst.
-      eapply H0.
-    }
+(* Each index has an associate datatype.  Let's name each one. *)
+Definition TBookStorage := BagType BookStorage.
+Definition TOrderStorage := BagType OrderStorage.
 
-    hone method "AddBook".
-    {
-      rewrite refine_pick_val with (A := nat) (a := length (fst r_n)).
-      simplify with monad laws.
-      rewrite refine_tupleAgree_refl_True;
-        simplify with monad laws.
-      (* Again, to tactics *)
-      repeat match goal with
-          |- context [
-                 forall tup' : @IndexedTuple ?h,
-                   (?qs ! ?R )%QueryImpl tup' ->
-                   tupleAgree ?n (indexedTuple tup') ?attrlist2%SchemaConstraints ->
-                   tupleAgree ?n (indexedTuple tup') ?attrlist1%SchemaConstraints ]
-              =>
-              let H' := fresh in
-              generalize (@refine_unused_key_check h attrlist1 attrlist2 _ _ n (qs ! R )%QueryImpl) as H'; intros; setoid_rewrite H'; clear H';
-              [ simplify with monad laws |
-                unfold BookStoreListImpl_AbsR in *; split_and; eauto ]
-        | |- context [
-                 forall tup' : @IndexedTuple ?h,
-                   (?qs ! ?R )%QueryImpl tup' ->
-                   tupleAgree (indexedTuple tup') ?n ?attrlist2%SchemaConstraints ->
-                   tupleAgree (indexedTuple tup') ?n  ?attrlist1%SchemaConstraints]
-                =>
-                let H' := fresh in
-                generalize (@refine_unused_key_check' h attrlist1 attrlist2 _ _ n (qs ! R )%QueryImpl) as H'; intros; setoid_rewrite H'; clear H';
-                  [ simplify with monad laws |
-                    unfold BookStoreListImpl_AbsR in *; split_and; eauto ]
-      end.
-      pose_string_ids.
-      unfold BookStoreListImpl_AbsR in *; split_and; simpl.
-      rewrite refineEquiv_pick_pair.
-      simplify with monad laws; simpl.
-      Split Constraint Checks.
-      (* TODO move this back to a tactic *)
-      subst_strings; setoid_rewrite (@ImplementListInsert_eq); eauto.
-      simplify with monad laws.
-      match goal with
-          |- context
-               [{a | EnsembleIndexedListEquivalence
-                       ((@UpdateUnConstrRelation ?QSSchema ?c ?Ridx
-                                                (EnsembleInsert ?n (?c!?R)))!?R')%QueryImpl a}%comp] =>
-          let H := fresh in
-          generalize ((@ImplementListInsert_neq QSSchema
-                                                {| bindex := R' |}
-                                                {| bindex := R |} n c)) as H; intros; setoid_rewrite H
-      end; try reflexivity; try eassumption.
-      congruence.
-      rewrite refine_pick_val; eauto;
-      simplify with monad laws.
-      rewrite refine_pick_val; eauto;
-      simplify with monad laws.
-      reflexivity.
-      rewrite refine_pick_val; eauto;
-      simplify with monad laws.
-      rewrite refine_pick_val; eauto;
-      simplify with monad laws.
-      reflexivity.
-      intros.
-      destruct H0 as [[l l'] _].
-      generalize (l _ H1).
-      unfold not; intros.
-      eapply lt_irrefl.
-      destruct tup; simpl in *; subst.
-      eapply H0.
-    }
+(* This abstraction relation connects:
+ * 1. Abstract database from reference implementation, using sets
+ * 2. Our fancy realization, using search trees (from Bags library) *)
+Definition BookStoreListImpl_AbsR
+           (or : UnConstrQueryStructure BookStoreSchema)
+           (nr : TBookStorage * TOrderStorage) : Prop :=
+  or!sBOOKS ≃ benumerate (fst nr) /\ or!sORDERS ≃ benumerate (snd nr).
 
-    hone method "GetTitles".
-    {
-      simpl.
-      unfold BookStoreListImpl_AbsR in *; split_and.
-      pose_string_ids.
-      simplify with monad laws.
-      rewrite refine_List_Query_In; eauto.
-      subst_strings; rewrite refine_List_Query_In_Where.
-      rewrite refine_List_For_Query_In_Return;
-        simplify with monad laws; simpl.
-
-      setoid_rewrite refineEquiv_pick_pair.
-      pose_string_ids.
-      simplify with monad laws.
-      rewrite refine_pick_val by eassumption.
-      simplify with monad laws.
-      rewrite refine_pick_val by eassumption.
-      simplify with monad laws.
-      finish honing.
-  }
-
-    hone method "NumOrders".
-    {
-      simpl; unfold BookStoreListImpl_AbsR in *; split_and.
-      pose_string_ids.
-      simplify with monad laws.
-      subst_strings.
-      rewrite refine_List_Query_In; eauto.
-      rewrite refine_Join_List_Query_In; eauto.
-      rewrite refine_List_Query_In_Where.
-      rewrite refine_List_Query_In_Where.
-      rewrite refine_List_For_Query_In_Return.
-      rewrite refine_Count.
-      pose_string_ids.
-      simplify with monad laws; simpl.
-
-      setoid_rewrite refineEquiv_pick_pair.
-      simplify with monad laws.
-      rewrite refine_pick_val by eassumption.
-      simplify with monad laws.
-      rewrite refine_pick_val by eassumption.
-      simplify with monad laws.
-      finish honing.
-  }
-
-  hone constructor "InitBookstore".
-  { simplify with monad laws.
-    simpl; unfold BookStoreListImpl_AbsR in *;
-    pose_string_ids.
-    rewrite refineEquiv_pick_pair.
-    rewrite refine_pick_val by
-        apply EnsembleIndexedListEquivalence_Empty;
-    simplify with monad laws.
-    rewrite refine_pick_val by
-        apply EnsembleIndexedListEquivalence_Empty;
-      simplify with monad laws.
-    finish honing.
-  }
-
+Definition BookStore :
+  Sharpened BookStoreSpec.
+Proof.
+  plan BookStoreListImpl_AbsR.
   finish sharpening.
-  Defined.
-End BookStoreExamples.
+Defined.
