examples/Bookstore.verbose.v
@@ -1,0 +1,291 @@
+Section BookStoreExamples.
+  Require Import QueryStructureNotations.
+  Require Import ListImplementation.
+
+  (* Our bookstore has two relations (tables):
+     - The [Books] relation contains the books in the
+       inventory, represented as a tuple with
+       [Author], [Title], and [ISBN] attributes.
+       The [ISBN] attribute is a key for the relation,
+       specified by the [where attributes .. depend on ..]
+       constraint.
+     - The [Orders] relation contains the orders that
+       have been placed, represented as a tuple with the
+       [ISBN] and [Date] attributes.
+
+     The schema for the entire query structure specifies that
+     the [ISBN] attribute of [Orders] is a foreign key into
+     [Books], specified by the [attribute .. of .. references ..]
+     constraint.
+   *)
+
+  Definition BookStoreSchema :=
+    Query Structure Schema
+      [ relation "Books" has
+                schema <"Author" :: string,
+                        "Title" :: string,
+                        "ISBN" :: nat>
+                        where attributes ["Title"; "Author"] depend on ["ISBN"];
+        relation "Orders" has
+                schema <"ISBN" :: nat,
+                        "Date" :: nat> ]
+      enforcing [attribute "ISBN" for "Orders" references "Books"].
+
+  (* Aliases for the tuples contained in Books and Orders, respectively. *)
+  Definition Book := TupleDef BookStoreSchema "Books".
+  Definition Order := TupleDef BookStoreSchema "Orders".
+
+  (* Our bookstore has two mutators:
+     - [PlaceOrder] : Place an order into the 'Orders' table
+     - [AddBook] : Add a book to the inventory
+
+     Our bookstore has two observers:
+     - [GetTitles] : The titles of books written by a given author
+     - [NumOrders] : The number of orders for a given author
+   *)
+
+  Definition BookStoreSig : ADTSig :=
+    ADTsignature {
+        "InitBookstore" : unit → rep,
+        "PlaceOrder" : rep × Order → rep × bool,
+        "AddBook" : rep × Book → rep × bool,
+        "GetTitles" : rep × string → rep × list string,
+        "NumOrders" : rep × string → rep × nat
+      }.
+
+  Definition BookStoreSpec : ADT BookStoreSig :=
+    QueryADTRep BookStoreSchema {
+      const "InitBookstore" (_ : unit) : rep := empty,
+
+      update "PlaceOrder" ( o : Order ) : bool :=
+          Insert o into "Orders",
+
+      update "AddBook" ( b : Book ) : bool :=
+          Insert b into "Books" ,
+
+      query "GetTitles" ( author : string ) : list string :=
+        For (b in "Books")
+        Where (author = b!"Author")
+        Return (b!"Title"),
+
+       query "NumOrders" ( author : string ) : nat :=
+          Count (For (o in "Orders") (b in "Books")
+                 Where (author = b!"Author")
+                 Where (b!"ISBN" = o!"ISBN")
+                 Return o!"ISBN")
+  }.
+
+  Require Import BagsOfTuples.
+
+  Definition BookStoreListImpl_AbsR
+             (or : UnConstrQueryStructure BookStoreSchema)
+             (nr : list Book * list Order) : Prop :=
+    or ! "Books" ≃ benumerate (fst nr) /\ or ! "Orders" ≃ benumerate (snd nr).
+
+  Opaque Query_For.
+
+  Definition BookStore :
+    Sharpened BookStoreSpec.
+  Proof.
+    unfold BookStoreSpec.
+
+    (* Step 1: Drop the constraints on the tables. From the perspective
+      of a client of a sharpened ADT the invariants will still hold,
+      since ADT refinement preserves the simulation relation. *)
+
+    start honing QueryStructure.
+
+    hone representation using BookStoreListImpl_AbsR.
+
+    hone method "PlaceOrder".
+    {
+      rewrite refine_pick_val with (A := nat) (a := length (snd r_n)).
+      simplify with monad laws.
+      (* TODO: remove this etransitivity, apply step. *)
+      etransitivity.
+      apply refine_bind.
+      eapply (@refine_foreign_key_check
+                 _
+                 _ (fst r_n)
+      (fun tup2 : Tuple => n ``("ISBN") = tup2 ``("ISBN"))).
+      destruct H0; eauto.
+      unfold pointwise_relation; intros.
+      higher_order_1_reflexivity.
+      (* END TODO*)
+      pose_string_ids.
+      simplify with monad laws.
+      unfold If_Then_Else; rewrite refine_if_bool_eta.
+      simplify with monad laws.
+      unfold BookStoreListImpl_AbsR in *; split_and; simpl in *.
+      pose_string_ids.
+      rewrite refineEquiv_pick_pair.
+      simplify with monad laws; simpl.
+      Split Constraint Checks.
+      (* TODO move this back to a tactic *)
+      etransitivity.
+      subst_strings.
+      match goal with
+          |- context
+               [{a | EnsembleIndexedListEquivalence
+                       ((@UpdateUnConstrRelation ?QSSchema ?c ?Ridx
+                                                (EnsembleInsert ?n (?c!?R)))!?R')%QueryImpl a}%comp] =>
+          let H := fresh in
+          generalize ((@ImplementListInsert_neq QSSchema
+                                                {| bindex := R' |}
+                                                {| bindex := R |} n c)) as H; intros; setoid_rewrite H
+      end; try reflexivity; try eassumption.
+      congruence.
+      simplify with monad laws.
+      match goal with
+          |- context
+               [{a | EnsembleIndexedListEquivalence
+                       ((@UpdateUnConstrRelation ?QSSchema ?c ?Ridx
+                                                (EnsembleInsert ?n (?c!?R)))!?R)%QueryImpl a}%comp] =>
+          let H := fresh in
+          generalize ((@ImplementListInsert_eq QSSchema
+                                                {| bindex := R |}
+                                                n c)) as H; intros; setoid_rewrite H
+      end; try reflexivity; try eassumption.
+      rewrite refine_pick_val; eauto.
+      simplify with monad laws.
+      rewrite refine_pick_val; eauto.
+      simplify with monad laws.
+      reflexivity.
+      intros.
+      destruct H0 as [_ [l l']].
+      generalize (l _ H1).
+      unfold not; intros.
+      eapply lt_irrefl.
+      destruct tup; simpl in *; subst.
+      eapply H0.
+    }
+
+    hone method "AddBook".
+    {
+      rewrite refine_pick_val with (A := nat) (a := length (fst r_n)).
+      simplify with monad laws.
+      rewrite refine_tupleAgree_refl_True;
+        simplify with monad laws.
+      (* Again, to tactics *)
+      repeat match goal with
+          |- context [
+                 forall tup' : @IndexedTuple ?h,
+                   (?qs ! ?R )%QueryImpl tup' ->
+                   tupleAgree ?n (indexedTuple tup') ?attrlist2%SchemaConstraints ->
+                   tupleAgree ?n (indexedTuple tup') ?attrlist1%SchemaConstraints ]
+              =>
+              let H' := fresh in
+              generalize (@refine_unused_key_check h attrlist1 attrlist2 _ _ n (qs ! R )%QueryImpl) as H'; intros; setoid_rewrite H'; clear H';
+              [ simplify with monad laws |
+                unfold BookStoreListImpl_AbsR in *; split_and; eauto ]
+        | |- context [
+                 forall tup' : @IndexedTuple ?h,
+                   (?qs ! ?R )%QueryImpl tup' ->
+                   tupleAgree (indexedTuple tup') ?n ?attrlist2%SchemaConstraints ->
+                   tupleAgree (indexedTuple tup') ?n  ?attrlist1%SchemaConstraints]
+                =>
+                let H' := fresh in
+                generalize (@refine_unused_key_check' h attrlist1 attrlist2 _ _ n (qs ! R )%QueryImpl) as H'; intros; setoid_rewrite H'; clear H';
+                  [ simplify with monad laws |
+                    unfold BookStoreListImpl_AbsR in *; split_and; eauto ]
+      end.
+      pose_string_ids.
+      unfold BookStoreListImpl_AbsR in *; split_and; simpl.
+      rewrite refineEquiv_pick_pair.
+      simplify with monad laws; simpl.
+      Split Constraint Checks.
+      (* TODO move this back to a tactic *)
+      subst_strings; setoid_rewrite (@ImplementListInsert_eq); eauto.
+      simplify with monad laws.
+      match goal with
+          |- context
+               [{a | EnsembleIndexedListEquivalence
+                       ((@UpdateUnConstrRelation ?QSSchema ?c ?Ridx
+                                                (EnsembleInsert ?n (?c!?R)))!?R')%QueryImpl a}%comp] =>
+          let H := fresh in
+          generalize ((@ImplementListInsert_neq QSSchema
+                                                {| bindex := R' |}
+                                                {| bindex := R |} n c)) as H; intros; setoid_rewrite H
+      end; try reflexivity; try eassumption.
+      congruence.
+      rewrite refine_pick_val; eauto;
+      simplify with monad laws.
+      rewrite refine_pick_val; eauto;
+      simplify with monad laws.
+      reflexivity.
+      rewrite refine_pick_val; eauto;
+      simplify with monad laws.
+      rewrite refine_pick_val; eauto;
+      simplify with monad laws.
+      reflexivity.
+      intros.
+      destruct H0 as [[l l'] _].
+      generalize (l _ H1).
+      unfold not; intros.
+      eapply lt_irrefl.
+      destruct tup; simpl in *; subst.
+      eapply H0.
+    }
+
+    hone method "GetTitles".
+    {
+      simpl.
+      unfold BookStoreListImpl_AbsR in *; split_and.
+      pose_string_ids.
+      simplify with monad laws.
+      rewrite refine_List_Query_In; eauto.
+      subst_strings; rewrite refine_List_Query_In_Where.
+      rewrite refine_List_For_Query_In_Return;
+        simplify with monad laws; simpl.
+
+      setoid_rewrite refineEquiv_pick_pair.
+      pose_string_ids.
+      simplify with monad laws.
+      rewrite refine_pick_val by eassumption.
+      simplify with monad laws.
+      rewrite refine_pick_val by eassumption.
+      simplify with monad laws.
+      finish honing.
+  }
+
+    hone method "NumOrders".
+    {
+      simpl; unfold BookStoreListImpl_AbsR in *; split_and.
+      pose_string_ids.
+      simplify with monad laws.
+      subst_strings.
+      rewrite refine_List_Query_In; eauto.
+      rewrite refine_Join_List_Query_In; eauto.
+      rewrite refine_List_Query_In_Where.
+      rewrite refine_List_Query_In_Where.
+      rewrite refine_List_For_Query_In_Return.
+      rewrite refine_Count.
+      pose_string_ids.
+      simplify with monad laws; simpl.
+
+      setoid_rewrite refineEquiv_pick_pair.
+      simplify with monad laws.
+      rewrite refine_pick_val by eassumption.
+      simplify with monad laws.
+      rewrite refine_pick_val by eassumption.
+      simplify with monad laws.
+      finish honing.
+  }
+
+  hone constructor "InitBookstore".
+  { simplify with monad laws.
+    simpl; unfold BookStoreListImpl_AbsR in *;
+    pose_string_ids.
+    rewrite refineEquiv_pick_pair.
+    rewrite refine_pick_val by
+        apply EnsembleIndexedListEquivalence_Empty;
+    simplify with monad laws.
+    rewrite refine_pick_val by
+        apply EnsembleIndexedListEquivalence_Empty;
+      simplify with monad laws.
+    finish honing.
+  }
+
+  finish sharpening.
+  Defined.
+End BookStoreExamples.
